Added addEdge and findNode functions to generic finite graphs

examples/generic_finite_graphs/gfgScript.sml
@@ -1,10 +1,12 @@
-open HolKernel Parse boolLib bossLib;
+open HolKernel Parse boolLib bossLib listTheory;
 
-open sptreeTheory arithmeticTheory
+open sptreeTheory arithmeticTheory;
 
 val _ = new_theory "gfg";
 
 val _ = ParseExtras.tight_equality()
+val _ = monadsyntax.temp_add_monadsyntax();
+val _ = overload_on("monad_bind",``OPTION_BIND``);
 
 val _ = Datatype‘
   gfg = <| nodeInfo : α spt ;
@@ -22,11 +24,23 @@ val addNode_def = Define‘
                           followers updated_by (insert g.next []) ;
                           preds updated_by (insert g.next []) ; |>’;
 
+val addEdge_def = Define`
+  addEdge id (e,suc) g =
+     if (id ∈ domain g.nodeInfo) ∧ (suc ∈ domain g.nodeInfo)
+     then do followers_old <- lookup id g.followers;
+             SOME (g with <| followers updated_by
+                     (insert id ((e,suc)::followers_old))|>)
+          od
+     else NONE`;
+
+val findNode_def = Define`
+  findNode P g =
+    OPTION_MAP FST (FIND P (toAList g.nodeInfo))`;
+
 val wfAdjacency_def = Define‘
   wfAdjacency adjmap ⇔
      ∀k nl e n. lookup k adjmap = SOME nl ∧ MEM (e,n) nl ⇒
                 n ∈ domain adjmap’;
-
 
 val wfg_def = Define‘
   wfg g ⇔ (∀n. g.next ≤ n ⇒ n ∉ domain g.nodeInfo) ∧
@@ -43,6 +57,26 @@ val addNode_preserves_wfg = Q.store_thm(
   ‘wfg g ⇒ wfg (addNode i g)’,
   simp[wfg_def, addNode_def] >>
   dsimp[wfAdjacency_def, lookup_insert, cond_eq] >> metis_tac[]);
+
+val addEdge_preserves_wfg = Q.store_thm(
+   "addEdge_preserves_wfg[simp]",
+   `wfg g ∧ (addEdge i (e,s) g = SOME g2) ==> wfg g2`,
+   simp[wfg_def,addEdge_def] >>
+   dsimp[wfAdjacency_def, lookup_insert] >> rpt strip_tac
+   >> rw[] >> fs[]
+    >- metis_tac[]
+    >- (fs[INSERT_DEF,SET_EQ_SUBSET,SUBSET_DEF] >> rpt strip_tac
+          >> metis_tac[])
+    >- (rw[] >> fs[lookup_insert] >> Cases_on `k=i` >> fs[]
+        >- (Cases_on `MEM (e',n) followers_old`
+          >- metis_tac[]
+          >- (`(e',n) = (e,s)` by (rw[] >> fs[MEM])
+              >> rw[] >> fs[])
+          )
+        >- (fs[] >> metis_tac[])
+       )
+    >- metis_tac[]
+    );
 
 val graph_size_def = Define‘graph_size g = sptree$size g.nodeInfo’;
 
